src/base.v
@@ -1,0 +1,7 @@
+From stdpp Require Export base tactics list options.
+From RecordUpdate Require Export RecordUpdate.
+
+#[export] Set Printing Projections.
+
+Ltac simplify := repeat progress (intros; simpl in *; list_simplifier; subst).
+Ltac equality := intuition congruence.
