src/bitvector.v
@@ -1,0 +1,65 @@
+From research Require Import base.
+From stdpp Require Export bitvector.
+
+Local Open Scope bv_scope.
+
+(* This allows automation tactics such as [bv_solve] to assume lia can handle
+   `mod` and `div`. *)
+Ltac Zify.zify_post_hook ::= Z.div_mod_to_equations.
+
+Definition bv_eqb {n} (x y : bv n) : bool :=
+  Eval cbv delta [ bool_decide decide_rel ] in
+    bool_decide (x = y).
+
+Definition bv_odd {n} (x : bv n) := Z.odd (bv_unsigned x).
+
+Infix "=?" := bv_eqb : bv_scope.
+Infix "#" := bv_zero_extend (at level 65) : bv_scope.
+Infix "||" := (bv_concat _) : bv_scope.
+Notation "x ?" := (bv_odd x) : bv_scope.
+
+Lemma bv_eqb_eq {n} : forall (x y : bv n), (x =? y) = true <-> x = y.
+Proof.
+  intuition; simplify.
+  - unfold bv_eqb in *. destruct (bv_eq_dec n x y); equality.
+  - unfold bv_eqb. destruct (bv_eq_dec n y y); equality.
+Qed.
+
+Lemma bv_eqb_neq {n} : forall (x y : bv n), (x =? y) = false <-> x <> y.
+Proof.
+  intuition; simplify.
+  - unfold bv_eqb in *. destruct (bv_eq_dec n y y); equality.
+  - unfold bv_eqb. destruct (bv_eq_dec n x y); equality.
+Qed.
+
+Lemma bv_not_zero_one : forall (x : bv 1), x <> 0 <-> x = 1.
+Proof.
+  simplify.
+  assert (x = 0 \/ x = 1).
+  { apply bv_1_ind with (P := (fun x => x = 0 \/ x = 1)); equality. }
+  split; simplify.
+  - destruct_or!; equality.
+  - destruct_or!; equality.
+Qed.
+
+Lemma bv_not_one_zero : forall (x : bv 1), x <> 1 <-> x = 0.
+Proof.
+  simplify.
+  assert (x = 0 \/ x = 1).
+  { apply bv_1_ind with (P := (fun x => x = 0 \/ x = 1)); equality. }
+  split; simplify.
+  - destruct_or!; equality.
+  - destruct_or!; equality.
+Qed.
+
+Ltac simplify_bv_eqb :=
+  repeat progress (
+      match goal with
+      | H: (?x =? 0) = true |- _ => rewrite bv_eqb_eq in H
+      | H: (?x =? 1) = true |- _ => rewrite bv_eqb_eq in H
+      | H: (?x =? 0) = false |- _ => rewrite bv_eqb_neq in H
+      | H: ?x <> 0 |- _ => rewrite bv_not_zero_one in H
+      | H: (?x =? 1) = false |- _ => rewrite bv_eqb_neq in H
+      | H: ?x <> 1 |- _ => rewrite bv_not_one_zero in H
+      end
+    ).
